experiments/Veritas.HashSet.fst
@@ -103,6 +103,8 @@ let add s b l =
   pop_frame ()
 #pop-options
 
+//let get s l =
+
 let free s =
   let { seen; acc; key } = !* s in
   B.free s;
